src/SeqDisk/AsyncReplicatedDisk.v
@@ -3,7 +3,9 @@ Require Import Disk.AsyncDisk.
 
 Require Import Refinement.ProgLang.Prog.
 Require Import Refinement.ProgLang.Hoare.
-Require Import TwoDisk.AsyncTwoDiskAPI.
+Require Import
+        TwoDisk.AsyncTwoDiskAPI
+        TwoDisk.AsyncTwoDiskTheorems.
 Require Import SeqDisk.AsyncDiskAPI.
 
 Require Import SeqDisk.AsyncReplicatedDisk.Step.
@@ -181,6 +183,215 @@ Module RD.
         right.
         intuition eauto using pred_weaken.
     Qed.
+
+    Theorem DiskSize_rok :
+      prog_spec
+        (fun d state =>
+           {|
+             pre := TD.disk0 state |= covered d /\
+                    TD.disk1 state |= covered d;
+             post :=
+               fun r state' =>
+                 r = size d /\
+                 TD.disk0 state' |= covered d /\
+                 TD.disk1 state' |= covered d;
+             recover :=
+               fun _ state' =>
+                 TD.disk0 state' |= crashesTo d /\
+                 TD.disk1 state' |= crashesTo d;
+           |})
+        (DiskSize td) (_ <- irec td; Recover td)
+        (refinement td).
+    Proof.
+      start.
+
+      rename a into d.
+      descend; (intuition eauto); simplify.
+      descend; (intuition eauto); simplify.
+      eapply pred_weaken; eauto.
+      eapply pred_weaken; eauto.
+    Qed.
+
+    Theorem Sync_rok :
+      prog_spec
+        (fun d state =>
+           {|
+             pre := TD.disk0 state |= covered d /\
+                    TD.disk1 state |= covered d;
+             post :=
+               fun r state' =>
+                 r = tt /\
+                 TD.disk0 state' |= then_flush (covered d) /\
+                 TD.disk1 state' |= then_flush (covered d);
+             recover :=
+               fun _ state' =>
+                 TD.disk0 state' |= crashesTo d /\
+                 TD.disk1 state' |= crashesTo d;
+           |})
+        (Sync td) (_ <- irec td; Recover td)
+        (refinement td).
+    Proof.
+      start.
+
+      rename a into d.
+      descend; (intuition eauto); simplify.
+      - descend; (intuition eauto); simplify.
+        eauto using pred_weaken.
+        eauto using pred_weaken.
+      - descend; (intuition eauto); simplify.
+        all: admit. (* need to show crashesTo is weaker than then_flush
+        (flushing is one possible crash state, so this should be true) *)
+      - descend; (intuition eauto); simplify.
+        all: admit.
+    Admitted.
+
+    (* Now we gather up the implementation and all the correctness proofs,
+    expressing them in terms of the high-level API in D.API. *)
+
+    (* First, we prove some lemmas that re-express the D.API semantics in more
+    convenient terms (in some cases, just for the sake of the automation). *)
+
+    Lemma read_step : forall a (state state':D.State) b,
+        state a |= (fun bs => curr_val bs = b) ->
+        state' = state ->
+        D.step (D.Read a) state b state'.
+    Proof.
+      intros; subst.
+      constructor; auto.
+      intros.
+      replace (state a) in *; auto.
+    Qed.
+
+    Lemma write_step : forall a b (state state':D.State) u,
+        state' = diskUpdF state a (buffer b) ->
+        D.step (D.Write a b) state u state'.
+    Proof.
+      intros; subst.
+      destruct u.
+      econstructor; eauto.
+    Qed.
+
+    Lemma sync_step : forall (state state':D.State) u,
+        state' = flush state ->
+        D.step (D.Sync) state u state'.
+    Proof.
+      intros; subst.
+      destruct u.
+      econstructor; eauto.
+    Qed.
+
+    Lemma disk_size_step : forall (state state':D.State) r,
+        r = size state ->
+        state' = state ->
+        D.step (D.DiskSize) state r state'.
+    Proof.
+      intros; subst.
+      econstructor; eauto.
+    Qed.
+
+    Hint Resolve read_step write_step sync_step disk_size_step.
+
+    (* The proof will require a refinement; we build one up based on the
+    two-disk state. *)
+
+    (* TODO: fix [D.State] to allow two durable values *)
+    Definition rd_abstraction (state:TD.State) : D.State :=
+      match state with
+      | TD.Disks (Some d) _ _ => d
+      | TD.Disks None (Some d) _ => d
+      | _ => empty_disk (* impossible *)
+      end.
+
+    Definition rd_invariant (state:TD.State) :=
+      match state with
+      | TD.Disks (Some d_0) (Some d_1) _ =>
+        d_0 = d_1
+      | _ => True
+      end.
+
+    (* Finally, we put together the pieces of the [Interface]. Here we also
+    convert from our specificatiosn above to the exact form that an Interface
+    uses; the proofs are automatic after defining the lemmas above about D.step
+    and the layer refinement. *)
+
+    Definition d_op_impl T (op:D.Op T) : prog T :=
+      match op with
+      | D.Read a => Read td a
+      | D.Write a b => Write td a b
+      | D.Sync => Sync td
+      | D.DiskSize => DiskSize td
+      end.
+
+    Definition rd_refinement :=
+      refinement_compose
+        (refinement td)
+        {| invariant := rd_invariant;
+           abstraction := rd_abstraction; |}.
+
+    Definition impl : InterfaceImpl D.Op :=
+      {| op_impl := d_op_impl;
+         recover_impl := _ <- irec td; Recover td;
+         init_impl := then_init (iInit td) (Init td) |}.
+
+    Hint Resolve Read_rok Write_rok Sync_rok DiskSize_rok Recover_rok.
+
+    Theorem state_some_disks : forall state,
+        exists d_0 d_1,
+          TD.disk0 state |= eq d_0 /\
+          TD.disk1 state |= eq d_1.
+    Proof.
+      destruct state.
+      destruct disk0, disk1; simpl; eauto.
+      exfalso; eauto.
+    Qed.
+
+    Theorem rd_crash_effect_valid :
+      crash_effect_valid {| invariant := rd_invariant;
+                            abstraction := rd_abstraction |}
+                         TD.wipe D.wipe.
+    Proof.
+      econstructor; intros; simpl.
+      - unfold rd_abstraction.
+        destruct w; simpl.
+        destruct disk0, disk1; auto.
+        exfalso; eauto.
+      - eapply diskMem_ext_eq.
+        extensionality a.
+        simpl.
+        destruct matches.
+    Qed.
+
+    Definition rd : Interface D.API.
+      unshelve econstructor.
+      - exact impl.
+      - exact rd_refinement.
+      - intros.
+        destruct op; unfold op_spec;
+          apply spec_refinement_compose;
+          eapply prog_spec_weaken; eauto;
+            unfold spec_impl; simplify.
+        + exists (mapDisk (rd_abstraction state)
+                     (fun bs => {| current_val := curr_val bs;
+                                durable_vals := durable_val bs::nil; |})).
+          (intuition eauto); simplify.
+          all: admit.
+        + all: admit.
+        + all: admit.
+        + all: admit.
+      - eapply rec_noop_compose; eauto; simpl.
+        apply rd_crash_effect_valid.
+        eapply prog_spec_weaken; eauto;
+          unfold spec_impl; simplify.
+        unfold crash_invariant in *; simpl in *; repeat deex.
+        admit.
+      - eapply then_init_compose; eauto.
+        eapply prog_spec_weaken; unfold spec_impl; simplify.
+        admit.
+      - eapply crash_effect_compose; unfold wipe_valid;
+          eauto using crash_effect_ok; simpl; intros.
+        apply rd_crash_effect_valid.
+        apply rd_crash_effect_valid.
+    Admitted.
 
   End ReplicatedDisk.
 
